Refactor callbacks; refactor dwt and vst enc; [skip ci]

src/Lib/VstLib.v
@@ -5,30 +5,20 @@ Require Import Lib.
 
 Require Export Lib.
 
-Instance CompSpecs : compspecs. make_compspecs prog. Defined.
-
-(* memory representation of abstract types *)
-Parameter TYPE_descriptor_rep : TYPE_descriptor
-                                -> reptype (Tstruct _asn_TYPE_descriptor_s noattr). 
-
-(* These two will express memory specifications *)
-
-(* on any error write {buf = 0; size = 0},
-    else {buf = ls; size = |ls|}*)
-Parameter PRIMITIVE_TYPE_rep : option byte
-                               -> reptype (Tstruct _ASN__PRIMITIVE_TYPE_s noattr).
-
 Definition cb_type := (Tfunction 
                           (Tcons (tptr tvoid) 
                                  (Tcons tuint (Tcons (tptr tvoid) Tnil))) tint 
                           cc_default).
-Definition enc_rval_s := Tstruct _asn_enc_rval_s noattr.
 Definition type_descriptor_s := Tstruct _asn_TYPE_descriptor_s noattr.
 Definition asn_codec_ctx_s := Tstruct _asn_codec_ctx_s noattr.
-Definition asn_dec_rval_s := Tstruct _asn_dec_rval_s noattr.
 
-Definition construct_enc_rval encoded (sptr : val) := 
+(* Encoder return struct *)
+Definition enc_rval_s := Tstruct _asn_enc_rval_s noattr.
+Definition mk_enc_rval encoded (sptr : val) := 
   (Vint (Int.repr encoded), (Vundef, sptr)).
 
-Definition construct_dec_rval code consumed := 
+(* Decoder return struct *)
+Definition asn_dec_rval_s := Tstruct _asn_dec_rval_s noattr.
+Definition mk_dec_rval code consumed := 
   (Vint (Int.repr code), Vint (Int.repr consumed)).
+
