src/Lib/Callback/Dummy.v
@@ -1,0 +1,23 @@
+Require Import Core.Core Core.Tactics.
+Require Import VST.floyd.proofauto.
+Require Import VST.floyd.library.
+Require Import Clight.asn_application.
+Require Import Lib.VstLib Lib.Stdlib.
+Require Import Core.Notations.
+
+Instance CompSpecs : compspecs. make_compspecs prog. Defined.
+
+Open Scope Z.
+
+Definition dummy_callback  : funspec :=
+    WITH  data_p : val, size : Z,
+         key_p : val
+    PRE [tptr tvoid, tuint, tptr tvoid]
+      PROP ()
+      PARAMS (data_p; Vint (Int.repr size); key_p)
+      GLOBALS ()
+      SEP ()
+    POST [tint]
+      PROP ()
+      LOCAL (temp ret_temp Vzero)
+      SEP (). 
