src/Lib/Callback/Overrun.v
@@ -1,0 +1,102 @@
+Require Import Core.Core Core.Tactics.
+Require Import VST.floyd.proofauto.
+Require Import VST.floyd.library.
+Require Import Clight.asn_application.
+Require Import Lib.VstLib Lib.Stdlib.
+Require Import Core.Notations.
+
+Instance CompSpecs : compspecs. make_compspecs prog. Defined.
+
+Open Scope Z.
+
+(* Overrun callback key *)
+Definition enc_key_s := Tstruct _overrun_encoder_key noattr.
+Definition mk_enc_key buf size comp_size : reptype enc_key_s := 
+  (buf, (Vint (Int.repr size), Vint (Int.repr comp_size))). 
+
+Definition callback  : funspec :=
+    WITH (* parameters *)
+         data : list int, data_p : val, 
+         size : Z,
+         key_p : val, 
+         (* overrun_encoder_key fields *)
+         buf_p : val,
+         buf_size : Z, computed_size : Z
+    PRE [tptr tvoid, tuint, tptr tvoid]
+      PROP (size = Zlength data;
+            0 <= buf_size <= Int.max_unsigned;
+            0 <= computed_size <= Int.max_unsigned;
+            0 <= size <= Int.max_unsigned;
+            0 <= computed_size + size <= Int.max_unsigned;
+            isptr buf_p)
+      PARAMS (data_p; Vint (Int.repr size); key_p)
+      GLOBALS ()
+      SEP (data_at Tsh (tarray tuchar (Zlength data)) (map Vint data) data_p;
+           data_at Tsh enc_key_s 
+                   (mk_enc_key buf_p buf_size computed_size) 
+                   key_p;
+          if buf_size <? computed_size + size 
+          then emp
+          else memory_block Tsh size (offset_val computed_size buf_p))    
+     POST [tint]
+      PROP ()
+      LOCAL (temp ret_temp Vzero)
+      SEP (data_at Tsh (tarray tuchar (Zlength data)) (map Vint data) data_p;
+           if buf_size <? computed_size + size 
+           then data_at Tsh enc_key_s 
+                   (mk_enc_key buf_p 0 (computed_size + size))  
+                   key_p
+           else 
+             (data_at Tsh (tarray tuchar size) (map Vint data) 
+                      (offset_val computed_size buf_p) *
+              data_at Tsh enc_key_s 
+                      (mk_enc_key buf_p buf_size (computed_size + size)) key_p)). 
+
+Definition callback_overrun_spec : ident * funspec :=
+  DECLARE _overrun_encoder_cb callback.
+
+Definition Vprog : varspecs. mk_varspecs prog. Defined.
+Definition Gprog := ltac:(with_library prog [callback_overrun_spec; 
+                                             (_memcpy, memcpy_spec)]).
+
+Theorem bool_der_encode : semax_body Vprog Gprog f_overrun_encoder_cb 
+                                     callback_overrun_spec.
+Proof.
+  start_function.
+  destruct (buf_size <? computed_size + size) eqn : Q.
+  - repeat forward. 
+    assert (buf_size < computed_size + size) by (Zbool_to_Prop; eassumption).
+    forward_if 
+      (PROP ()
+            LOCAL (temp _t'3 (Vint (Int.repr buf_size)); 
+                   temp _t'2 (Vint (Int.repr computed_size));
+                   temp _key key_p; temp _data data_p; 
+                   temp _size (Vint (Int.repr size));
+                   temp _keyp key_p)
+            SEP (data_at Tsh (tarray tuchar (Zlength data)) (map Vint data) data_p;
+                 data_at Tsh enc_key_s 
+                         (mk_enc_key buf_p 0 computed_size) key_p));
+      repeat (forward || entailer! || nia).    
+  - assert (computed_size + size <= buf_size) by (Zbool_to_Prop; eassumption).
+    repeat forward.
+    unfold mk_enc_key.
+    forward_if
+      (PROP ()
+            LOCAL (
+              temp _t'5 (Vint (Int.repr computed_size)); 
+              temp _t'4 buf_p;
+              temp _t'3 (Vint (Int.repr buf_size)); 
+              temp _t'2 (Vint (Int.repr computed_size));
+              temp _key key_p; temp _data data_p; 
+              temp _size (Vint (Int.repr size));
+              temp _keyp key_p)
+            SEP (data_at Tsh (tarray tuchar (Zlength data)) (map Vint data) data_p;
+                 data_at Tsh (tarray tuchar size) (map Vint data) 
+                         (offset_val computed_size buf_p);
+                 data_at Tsh enc_key_s 
+                         (mk_enc_key buf_p buf_size (computed_size)) key_p));
+      repeat (forward || entailer! || nia). 
+    forward_call (Tsh, Tsh, offset_val computed_size buf_p, data_p, size, data);
+      entailer!.
+    cbn; entailer!.
+Qed.
